Proof Block correct

theories/Block.v
@@ -11,8 +11,50 @@ Definition blocks_aux (G: map_cfg) : _ -> (blk*map_cfg) := fun '(id, b) => (b, r
 
 Definition blocks (G: map_cfg): list (blk*map_cfg) := List.map (blocks_aux G) (elements G).
 
-Definition block_sem (G G': map_cfg) b := MapsTo_id b G /\ G' = (remove_id b G) /\ wf_map_cfg G'.
+Definition blocks_aux_sem (G0 G G': map_cfg) b :=
+  MapsTo_id b G /\ G' = (remove_id b G0) /\ wf_map_cfg G'.
 
-Lemma blocks_correct: forall G G' b, wf_map_cfg G -> ((b, G') ∈ (blocks G) <-> block_sem G G' b).
+Definition blocks_sem (G G': map_cfg) b := blocks_aux_sem G G G' b.
+
+Definition P G0 G := forall G' b, wf_map_cfg G -> wf_map_cfg G0 ->
+  ((b, G') ∈ (List.map (blocks_aux G0) (elements G))) <-> blocks_aux_sem G0 G G' b.
+
+Lemma blocks_aux_correct: forall G0 G, P G0 G.
 Proof.
-Admitted.
+  intros G0 G.
+  apply map_induction_min; unfold P.
+  - intros E He G' B Hwf Hwf0. split.
+    * assert (HE: elements E = []) by now apply elements_Empty. now rewrite HE.
+    * intros [HE _]. contradict HE. intro. eapply empty_mapsto_iff.
+      eapply MapsTo_m. reflexivity. reflexivity. symmetry. apply Eempty. apply He. apply H.
+  - intros G1 G2 Hrec idB B HBe HB G' A Hwf2 Hwf0. rewrite Add_add in HB. 
+    assert (HidB: B.(blk_id) = idB). {
+      apply Hwf2. eapply MapsTo_m. reflexivity. reflexivity. apply HB. now apply add_1.
+    } subst.
+    replace (elements G2) with ((B.(blk_id), B)::(elements G1)). 2: {
+      symmetry. apply eqlistA_eq. now apply elements_Add_Below.
+    } apply Below_In in HBe.
+    split. intros [H|H]. 3: case (eq_dec A.(blk_id) B.(blk_id)); unfold eq; intros He [HMA [HRA Hwf']].
+    * apply pair_equal_spec in H as []. subst A G'. 
+    repeat split; trivial.
+      + eapply MapsTo_m. reflexivity. reflexivity. apply HB. now apply add_1.
+      + now apply remove_wf_map_cfg.
+    * apply Hrec in H as [HMA [HRA Hwf']]; trivial.
+      assert (Hne: ~ A.(blk_id)===B.(blk_id)). { 
+        intro. apply HBe. exists A. eapply MapsTo_m. 4: apply HMA. now symmetry. reflexivity. reflexivity.
+      }
+      repeat split;trivial.
+      + eapply MapsTo_m. reflexivity. reflexivity. apply HB. apply add_2. now apply neq_sym. trivial.
+      + eapply wf_map_cfg_add. apply HBe. eapply wf_map_cfg_eq. apply HB. trivial.
+    * assert (Heq: A=B). { 
+      eapply wf_map_cfg_blk. apply Hwf2. apply HMA. eapply MapsTo_m.  apply He. reflexivity. apply HB. now apply add_1.
+    } subst. now left.
+    * right. apply Hrec; trivial. eapply wf_map_cfg_add. apply HBe. eapply wf_map_cfg_eq. apply HB. trivial.
+      repeat split; trivial.
+      eapply add_3. apply neq_sym. apply He. eapply MapsTo_m. reflexivity. reflexivity. symmetry. apply HB. trivial.
+Qed.
+
+Lemma blocks_correct: forall G G' b, wf_map_cfg G -> ((b, G') ∈ (blocks G) <-> blocks_sem G G' b).
+Proof.
+  intros. now apply blocks_aux_correct.
+Qed.
